Update lexer.dfy
Mostly verified -- still need to detect/ensure all tokens are valid or not

lexer.dfy
@@ -1,12 +1,44 @@
-
-//TODO might be good to separate the lexing parts from the parsing parts
-
 datatype TokenType = LEFT_PAREN | RIGHT_PAREN | DOT | MINUS | PLUS | STAR | SLASH 
-                     | UNARY_OP | BINARY_OP | VARIABLE_OP | NUMBER | EOF
+                     | UNARY_OP | BINARY_OP | VARIABLE_OP | NUMBER | EOF | TEMPSTRING
 
 datatype Token = Pair(token_type:TokenType, token_value:string)
 
-method Sum(str: seq<char>) returns (tokenized: seq<Token>)
+
+predicate validtype(token: Token){
+    token.token_type==LEFT_PAREN ||
+    token.token_type==RIGHT_PAREN ||
+    token.token_type==MINUS ||
+    token.token_type==PLUS ||
+    token.token_type==STAR ||
+    token.token_type==SLASH ||
+    token.token_type==NUMBER ||
+    token.token_type==UNARY_OP ||
+    token.token_type==BINARY_OP ||
+    token.token_type==VARIABLE_OP ||
+    token.token_type==EOF
+}
+function Flatten(tok: seq<Token>): seq<char>
+{
+    if |tok|==0 then []
+    else Flatten(tok[0..|tok|-1])+tok[|tok|-1].token_value
+  
+}
+lemma Flatsame(tok: seq<Token>,tok2: seq<Token>)
+requires |tok|==|tok2|
+requires forall i :: 0<=i<|tok| ==> tok[i].token_value==tok2[i].token_value;
+ensures Flatten(tok)==Flatten(tok2);
+{
+
+}
+
+/*predicate matchesString(str: seq<char>,tokenized: seq<Token>){
+    forall i :: 0<=i<|str| ==> 
+    (
+        
+    )
+}*/
+
+method Lex(str: seq<char>) returns (tokenized: seq<Token>)
 requires forall i::0<=i<|str| ==> (
 (str[i] as int >=48 && str[i] as int  <=57) ||
 str[i]=='+' ||
@@ -17,13 +49,25 @@ str[i]=='(' ||
 str[i]==')'
 )
 
+
+//ensures no tempstrings
+ensures forall i:: 0<=i<|tokenized| ==> (validtype(tokenized[i]))
+
+//ensures all tokens are valid and correct type
+//ensures all characters are represented in order in tokens
+ensures Flatten(tokenized)==str;
+
 {
     var i:=0;
     //var tokpos:=0;
     var tok: seq<Token> := [];
-    while i<|str|{
+    while i<|str|
+    invariant forall i:: 0<=i<|tok| ==> (validtype(tok[i]) ||tok[i].token_type==TEMPSTRING)
+    invariant i<=|str|
+    invariant Flatten(tok)==str[0..i]
+    {
         //numbers
-        if (str[i] as int >=48 && str[i] as int  <=57){
+        if ((str[i] as int >=48 && str[i] as int  <=57) || str[i]=='.'){
             if(|tok|>=1 && tok[|tok|-1].token_type==NUMBER){ //if last is number
                 tok := tok[|tok|-1 :=   //add digit
                 Pair(NUMBER,tok[|tok|-1].token_value+[str[i]])];
@@ -32,30 +76,89 @@ str[i]==')'
                 tok:=tok + [Pair(NUMBER,[str[i]])];
             }
         }
+        //letters 97 to 122
+        else if (str[i] as int >=97 && str[i] as int  <=122){
+            if(|tok|>=1 && tok[|tok|-1].token_type==TEMPSTRING){ //if last is number
+                tok := tok[|tok|-1 :=   //add letter
+                Pair(NUMBER,tok[|tok|-1].token_value+[str[i]])];
+            }
+            else{
+                tok:=tok + [Pair(TEMPSTRING,[str[i]])];
+            }
+        }
         //basic symbols
         else{
             if(str[i]=='+'){
-                tok:=tok + [Pair(PLUS,"idk?")];
+                tok:=tok + [Pair(PLUS,"+")];
             }
             else if(str[i]=='-'){
-               tok:=tok + [Pair(MINUS,"idk?")];
+               tok:=tok + [Pair(MINUS,"-")];
             }
             else if(str[i]=='*'){
-               tok:=tok + [Pair(STAR,"idk?")];
+               tok:=tok + [Pair(STAR,"*")];
             }
             else if(str[i]=='/'){
-               tok:=tok + [Pair(SLASH,"idk?")];
+               tok:=tok + [Pair(SLASH,"/")];
             }
             else if(str[i]=='('){
-               tok:=tok + [Pair(LEFT_PAREN,"idk?")];
+               tok:=tok + [Pair(LEFT_PAREN,"(")];
             }
             else if(str[i]==')'){
-               tok:=tok + [Pair(RIGHT_PAREN,"idk?")];
+               tok:=tok + [Pair(RIGHT_PAREN,")")];
             }
             //tokpos:=tokpos+1;
             //num==0;
         }
+        assert validtype(tok[|tok|-1]) || tok[|tok|-1].token_type==TEMPSTRING;
+        i:=i+1;
+    }
+    //specifying strings
+    i:=0;
+    //assert i<=|tok|;
+    assert forall i:: 0<=i<|tok| ==> (validtype(tok[i]) ||tok[i].token_type==TEMPSTRING);
+    assert Flatten(tok)==str;
+    ghost var a:=tok;
+
+    while i<|tok|
+    invariant i<=|tok|
+    invariant forall i:: 0<=i<|tok| ==> (validtype(tok[i]) ||tok[i].token_type==TEMPSTRING);
+    invariant forall j:: 0<=j<i ==> ((validtype(tok[j])))
+    invariant |a|==|tok|
+    invariant forall i:: 0<=i<|tok| ==> a[i].token_value==tok[i].token_value;
+    invariant Flatten(tok)==str
+    {
+        //ghost var a:=tok[i];
+        //assert validtype(tok[i]) || tok[i].token_type==TEMPSTRING;
+        if(tok[i].token_type==TEMPSTRING){ //if token is string
+            
+            if(tok[i].token_value=="abs" || tok[i].token_value=="sqrt" || tok[i].token_value=="ceil"){
+                
+                tok := tok[i :=
+                Pair(UNARY_OP,tok[i].token_value)];
+                
+            }
+            else if(tok[i].token_value=="modulo" || tok[i].token_value=="expt"){
+                tok := tok[i :=
+                Pair(BINARY_OP,tok[i].token_value)];
+            }
+            else if(tok[i].token_value=="min" || tok[i].token_value=="max"){
+                tok := tok[i :=
+                Pair(VARIABLE_OP,tok[i].token_value)];
+            }
+            else{
+                //REMOVE THIS LATER
+                tok := tok[i :=
+                Pair(VARIABLE_OP,tok[i].token_value)];
+            }   
+        }
+        assert a[i].token_value==tok[i].token_value;
+        Flatsame(tok,a);
+        assert validtype(tok[i]);
         i:=i+1;
     }
     return tok;
 }
+
+/*match result_var
+           case Ok => do something;
+           case Err => do something else;*/
